Inductive generation (Fixpoint reasoning 2 ) (#64)
* witnessing_sequence_extend

* witnessed_elements_prefixpoint

* WIP breaks

* proof of witnessing_sequence_extend (extended)

* WIP

* proved

* move & fix

* witnessing_sequence_alt

* finish inductive generation

src/FixpointReasoning.v
@@ -10,7 +10,7 @@ From Coq.Logic Require Import PropExtensionality ClassicalFacts.
 
 From stdpp Require Import base list.
 
-From MatchingLogic Require Import Syntax Semantics DerivedOperators Helpers.monotonic Utils.Lattice.
+From MatchingLogic Require Import Syntax Semantics DerivedOperators Helpers.monotonic Utils.Lattice Utils.stdpp_ext.
 
 Section with_signature.
   Context {Σ : Signature}.
@@ -120,17 +120,18 @@ Section with_signature.
         apply pattern_interpretation_mu_lfp_fixpoint. apply Hwfp.
       + intros S. subst. apply pattern_interpretation_mu_lfp_least. apply Hwfp.
   Qed.
-  
+
+  (* mu X. base \/ step X *)
+  (* [Nats] = mu X. 0 \/ succ X *)
+  (* [Nats] = \{ x | \ex x0,x1,..x_n . x0 \in 0 /\ x(i+1) \in succ xi }*)
+  (*  0, 1, 2,... x*)
   Section inductive_generation.
     Context (base step : Pattern).
 
     Let patt_ind_gen_body := (patt_or (nest_mu base) (patt_app (nest_mu step) (patt_bound_svar 0))).
     Let patt_ind_gen_simple_body := (patt_or base (patt_app step (patt_free_svar (fresh_svar patt_ind_gen_body)))).
     
-    
     Definition patt_ind_gen := patt_mu patt_ind_gen_body.
-
-    Search svar_open nest_mu.
 
     Hypothesis (Hwfpbase : well_formed_positive base).
     Hypothesis (Hwfpstep : well_formed_positive step).
@@ -185,36 +186,257 @@ Section with_signature.
       Context (ρₛ : @SVarVal Σ M).
 
 
-      Let F := @Fassoc Σ M ρₑ ρₛ patt_ind_gen_simple_body (fresh_svar patt_ind_gen_body).
-      
+      Let F := let X := fresh_svar patt_ind_gen_body in
+               @Fassoc Σ M ρₑ ρₛ (svar_open 0 X patt_ind_gen_body) X.
+      (*
       Lemma svar_open_patt_ind_gen_body_assoc S:
         let X := fresh_svar patt_ind_gen_body in
         pattern_interpretation ρₑ (update_svar_val X S ρₛ) (svar_open 0 X patt_ind_gen_body)
         = F S.
-      Proof.
+      Proof. reflexivity.
+             (*
         cbv zeta.
         rewrite svar_open_patt_ind_gen_body_simpl.
         { apply set_svar_fresh_is_fresh. }
         subst F. unfold Fassoc.
+        rewrite svar_open_patt_ind_gen_body_simpl.
+        { apply set_svar_fresh_is_fresh.  }
+        reflexivity.*)
+      Qed.
+       *)
+
+      (* I can imagine this lemma to be proven automatically. *)
+      Lemma F_interp: F = λ A, Ensembles.Union _ (pattern_interpretation ρₑ ρₛ base)
+                                               (app_ext (pattern_interpretation ρₑ ρₛ step) A).
+      Proof.
+        unfold F. unfold Fassoc. apply functional_extensionality.
+        intros A. rewrite svar_open_patt_ind_gen_body_simpl.
+        { apply set_svar_fresh_is_fresh. }
+
+        rewrite pattern_interpretation_or_simpl.
+        rewrite pattern_interpretation_app_simpl.
+        rewrite pattern_interpretation_free_svar_simpl.
+        rewrite update_svar_val_same.
+        rewrite pattern_interpretation_free_svar_independent.
+        {
+          eapply svar_is_fresh_in_richer.
+          2: { apply set_svar_fresh_is_fresh. }
+          solve_free_svars_inclusion 5.
+        }
+        rewrite pattern_interpretation_free_svar_independent.
+        {
+          eapply svar_is_fresh_in_richer.
+          2: { apply set_svar_fresh_is_fresh. }
+          solve_free_svars_inclusion 5.
+        }
         reflexivity.
-      Qed.      
-
-      Definition witnessing_function := (λ (Acc : Prop * (Domain M)) new,
-                                         let (P, old) := Acc in
-                                         (app_ext
-                                            (@pattern_interpretation Σ M ρₑ ρₛ step)
-                                            (Ensembles.Singleton _ old)
-                                            new,
-                                          new)
-                                        ).
-
+      Qed.
+      
+      
       Definition is_witnessing_sequence (m : Domain M) (l : list (Domain M)) :=
         (last l = Some m) /\
         (match l with
          | [] => False
          | m₀::ms => (@pattern_interpretation Σ M ρₑ ρₛ base) m₀
-                     /\ fst (foldl witnessing_function (True, m₀) ms)
+(*                     /\ forall (n : nat), n <= length ms ->*)
+                                                             
+                     /\  (@Forall _
+                                  (λ (x : (Domain M) * (Domain M)),
+                                   let (old, new) := x in
+                                  app_ext
+                                    (@pattern_interpretation Σ M ρₑ ρₛ step)
+                                    (Ensembles.Singleton _ old)
+                                    new
+                                 )
+                                 (zip (m₀::ms) ms)
+                         )
+                           
          end).
+
+      Definition is_witnessing_sequence_alt (m : Domain M) (l : list (Domain M)) :=
+        (∃ lst, last l = Some lst /\ @pattern_interpretation Σ M ρₑ ρₛ base lst)
+          /\
+          hd_error l = Some m
+          /\
+          ((@Forall _
+                    (λ (x : (Domain M) * (Domain M)),
+                     let (new, old) := x in
+                     app_ext
+                       (@pattern_interpretation Σ M ρₑ ρₛ step)
+                       (Ensembles.Singleton _ old)
+                       new
+                    )
+                    (zip l (tail l))
+          )).
+
+      Lemma witnessing_sequence_alt_extend (m m' : Domain M) (l : list (Domain M)) :
+        (is_witnessing_sequence_alt m l
+         /\ (∃ step', pattern_interpretation ρₑ ρₛ step step' /\ app_interp step' m m')
+        ) <-> (is_witnessing_sequence_alt m' (m'::l) /\ l ≠ []).
+      Proof.
+        split.
+        - intros [[[lst [Hlst Hbase]] [Hhd Hwit]] [step' [Hstep' Hm']]].
+          split.
+          2: { destruct l. simpl in Hhd. inversion Hhd. discriminate. }
+          move: m Hhd m' step' Hm' Hstep'.
+          induction l; intros m Hhd m' step' Hm' Hstep'.
+          + simpl in Hhd. inversion Hhd.
+          + simpl in Hhd. inversion Hhd. subst a. clear Hhd.
+            unfold is_witnessing_sequence_alt.
+            destruct l.
+            { simpl in Hlst. inversion Hlst. subst m. clear Hlst.
+              split.
+              { exists lst. simpl. split. reflexivity. apply Hbase. }
+              simpl. split. reflexivity. apply Forall_cons.
+              split. exists step'. exists lst. split.
+              apply Hstep'. split. constructor. apply Hm'.
+              apply Forall_nil. exact I.
+            }
+            split.
+            { exists lst. split. simpl. simpl in Hlst. apply Hlst. apply Hbase. }
+            split.
+            { reflexivity. }
+            simpl in Hwit. simpl.
+            apply Forall_cons.
+            simpl in IHl. simpl in Hlst.
+            specialize (IHl Hlst).
+            inversion Hwit. subst. clear Hwit.
+            specialize (IHl H2). clear Hlst H2.
+            split.
+            { exists step'. exists m. split. apply Hstep'. split. constructor. apply Hm'. }
+            apply Forall_cons.
+            split.
+            { apply H1. }
+            specialize (IHl d).
+            specialize (IHl (eq_refl (Some d))).
+            destruct H1 as [step'' [d'' [Hstep'' [Hd'' Hstep''d'']]]].
+            inversion Hd''. subst d''. clear Hd''.
+            specialize (IHl m step'' Hstep''d'' Hstep'').
+            unfold is_witnessing_sequence_alt in IHl.
+            simpl in IHl.
+            destruct IHl as [_ [_ Hforall]].
+            inversion Hforall. subst. apply H2.
+        -            
+      Abort.
+            
+          
+
+
+      Lemma witnessing_sequence_extend
+            (m x m' : Domain M) (l : list (Domain M)):
+        (is_witnessing_sequence m (x::l) /\
+        ∃ step', (pattern_interpretation ρₑ ρₛ step step' /\
+        app_interp step' m m')) <->
+        (last (x::l) = Some m /\ is_witnessing_sequence m' ((x::l) ++ [m'])).
+      Proof.
+        split.
+        -
+          intros [Hwit [step' [Hstep' Hm']]].
+          destruct Hwit as [Hwit1 [Hwit2 Hwit3]].
+          split.
+          { apply Hwit1. }
+          split.
+          { apply last_snoc. }
+          simpl.
+          split.
+          { apply Hwit2. }
+          
+          destruct l.
+          { simpl. apply Forall_cons. split. 2: { apply Forall_nil. exact I. }
+            exists step'. exists x. split.
+            { apply Hstep'. }
+            split.
+            { constructor. }
+            simpl in Hwit1. inversion Hwit1. subst. apply Hm'.
+          }
+          simpl.
+          apply Forall_cons.
+          simpl in Hwit3. inversion Hwit3. subst. clear Hwit3.
+          rename H1 into Hd. rename H2 into Hwit.
+          split.
+          { apply Hd. } clear Hd.
+
+          move: d Hwit1 Hwit.
+          induction l.
+          + intros D Hm _.
+            simpl. simpl in Hm. inversion Hm. subst.
+            clear Hm.
+            apply Forall_cons.
+            split.
+            2: { apply Forall_nil. exact I. }
+            exists step'. exists m. split.
+            { apply Hstep'. }
+            split.
+            { constructor. }
+            apply Hm'.
+          + intros d Hlast Hwit. simpl.
+            inversion Hwit. subst.
+            apply Forall_cons.
+            split.
+            { apply H1. }
+            apply IHl. simpl in Hlast. simpl. apply Hlast.
+            apply H2.
+        - intros [Hlast H].
+          unfold is_witnessing_sequence in H.
+          destruct H as [_ H].
+          remember (length l) as len.
+          assert (Hlen: length l <= len).
+          { lia. }
+          clear Heqlen. simpl in H.
+          destruct H as [Hbase Hall].
+          unfold is_witnessing_sequence.
+          apply and_assoc.
+          split.
+          { apply Hlast. }
+          apply and_assoc.
+          split.
+          { apply Hbase. }
+          clear Hbase.
+          
+          move: x l Hlast Hall Hlen.
+          induction len.
+          + intros x l Hlast Hall Hlen.
+            destruct l.
+            2: { simpl in Hlen. lia.  }
+            simpl. simpl in Hall.
+            split.
+            { apply Forall_nil. exact I. }
+            inversion Hall. subst. clear Hall. clear H2.
+            destruct H1 as [step' [m'' [Hstep' [Hm'm'' Hstep'm'']]]].
+            inversion Hm'm''. subst. clear Hm'm''.
+            exists step'. split. apply Hstep'.
+            simpl in Hlast. inversion Hlast. subst.
+            apply Hstep'm''.
+          + intros x l Hlast Hall Hlen.
+            destruct l as [|x' l'].
+            { simpl in Hlast. inversion Hlast. clear Hlast. subst.
+              simpl in Hall.
+              inversion Hall. subst. clear Hall.
+              clear H2.
+              simpl.
+              split.
+              { apply Forall_nil. exact I. }
+              destruct H1 as [step' Hstep'].
+              exists step'.
+              destruct Hstep' as [m'' [Hstep' [Hmm'' Hm'']]].
+              split.
+              { apply Hstep'. }
+              inversion Hmm''. subst.
+              apply Hm''.
+            }
+            simpl in Hall. simpl in IHlen. simpl in Hlast.
+            inversion Hall. subst. clear Hall.
+            specialize (IHlen x' l' Hlast H2).
+            simpl.
+            rewrite Forall_cons.
+            apply and_assoc.
+            split.
+            { apply H1. }
+            apply IHlen.
+            simpl in Hlen. lia.
+      Qed.
+      
+      
 
       Definition witnessed_elements : Ensemble (Domain M) :=
         λ m, ∃ l, is_witnessing_sequence m l.
@@ -224,7 +446,7 @@ Section with_signature.
         unfold Included. unfold Ensembles.In.
         intros x Hx.
         unfold F in Hx. unfold Fassoc in Hx.
-        rewrite pattern_interpretation_or_simpl in Hx.
+        rewrite pattern_interpretation_or_simpl in Hx. fold svar_open in Hx. simpl in Hx.
         destruct Hx.
         - unfold Ensembles.In in H.
           unfold witnessed_elements.
@@ -239,6 +461,14 @@ Section with_signature.
             eapply svar_is_fresh_in_richer. 2: { subst. auto. }
             solve_free_svars_inclusion 5.
           }
+          simpl.
+          rewrite pattern_interpretation_svar_open_nest_mu' in H.
+          { 
+            eapply svar_is_fresh_in_richer.
+            2: { apply set_svar_fresh_is_fresh. }
+            simpl.
+            solve_free_svars_inclusion 2.
+          }
           assumption.
         - unfold Ensembles.In in H.
           rewrite pattern_interpretation_app_simpl in H.
@@ -248,43 +478,237 @@ Section with_signature.
           destruct H as [step' [m [H1 [H2 Happ]]]].
           unfold witnessed_elements in H2.
           destruct H2 as [l Hl].
-          unfold is_witnessing_sequence in Hl.
-          destruct Hl as [Hlast Hl].
-          destruct l as [|m₀ l'] eqn:Heql.
-          { contradiction. }
-          destruct Hl as [Hm₀ Hl].
 
           unfold witnessed_elements.
-          exists (l ++ [x]). unfold is_witnessing_sequence.
-          simpl. rewrite last_snoc.
-          split.
-          { reflexivity. }
-          rewrite Heql. simpl.
-          split.
-          { apply Hm₀. }
+          exists (l ++ [x]).
 
-          rewrite foldl_app. simpl.
-          assert (foldl witnessing_function (True, m₀) l' = (True, m)).
-          { rewrite (@surjective_pairing _ _ (foldl witnessing_function (True, m₀) l')).
-            rewrite (@surjective_pairing _ _ (True, m)).
-            simpl in Hl.
-            (* We need propositional extensionality here.
-               It would be better to reformulate *)
-            rewrite (provable_prop_ext propositional_extensionality _ Hl).
-            simpl.
-            admit. (*rewrite Hl.*)
-            
+          (* `l` is not empty *)
+          destruct l as [|m₀ l'] eqn:Heql.
+          { unfold is_witnessing_sequence in Hl. destruct Hl. simpl in H. inversion H. }
+
+          rewrite pattern_interpretation_svar_open_nest_mu in H1.
+          {
+            eapply svar_is_fresh_in_richer.
+            2: { apply set_svar_fresh_is_fresh. }
+            solve_free_svars_inclusion 2.
           }
-          rewrite H. simpl.
-          unfold app_ext.
-          exists step'. exists x.
-          admit.
-      Abort.
+
+          epose proof (P := @witnessing_sequence_extend _ _ _ _).
+          destruct P as [P _].
+          specialize (P (conj Hl (@ex_intro _ _ step' (conj H1 Happ)))).
+          apply P.
+      Qed.
+
+      Lemma interp_included_in_witnessed_elements:
+        Included _ (@pattern_interpretation Σ M ρₑ ρₛ patt_ind_gen) witnessed_elements.
+      Proof.
+        apply pattern_interpretation_mu_lfp_least.
+        { apply patt_ind_gen_wfp. }
+        apply witnessed_elements_prefixpoint.
+      Qed.
+
+      Lemma pattern_interpretation_patt_ind_gen_fix :
+        let Sfix := pattern_interpretation ρₑ ρₛ patt_ind_gen in
+        F Sfix = Sfix.
+      Proof.
+        apply pattern_interpretation_mu_lfp_fixpoint.
+        apply patt_ind_gen_wfp.
+      Qed.
+      
+      
+      Definition witnessed_elements_of_max_len len : Ensemble (Domain M) :=
+        λ m, ∃ l, is_witnessing_sequence m l /\ length l <= len.
+
+      Lemma witnessed_elements_of_max_len_included_in_interp len:
+        Included _ (witnessed_elements_of_max_len (S len)) (@pattern_interpretation Σ M ρₑ ρₛ patt_ind_gen).
+      Proof.
+        induction len.
+        - unfold Included. intros m.
+          rewrite -pattern_interpretation_patt_ind_gen_fix.
+          unfold Ensembles.In.
+          intros H.
+          unfold witnessed_elements_of_max_len.
+          rewrite F_interp.
+          destruct H as [l [Hwit Hlen]].
+          unfold is_witnessing_sequence in Hwit.
+          destruct Hwit as [Hlast Hm].
+          destruct l.
+          { simpl in Hlast. inversion Hlast. }
+          destruct l.
+          2: { simpl in Hlen. lia. }
+          simpl in Hlast. inversion Hlast. clear Hlast. subst.
+          destruct Hm as [Hm _].
+          left. unfold Ensembles.In. apply Hm.
+        - unfold Included. intros m.
+          rewrite -pattern_interpretation_patt_ind_gen_fix.
+          unfold Ensembles.In. intros H.
+          destruct H as [l [Hwit Hlen]].
+          unfold Included in IHlen. unfold Ensembles.In in IHlen.
+          rewrite F_interp.
+          pose proof (Hwit' := Hwit).
+          unfold is_witnessing_sequence in Hwit.
+          destruct Hwit as [Hlast Hl].
+          destruct l.
+          { contradiction. }
+          
+          simpl in Hlen.
+          destruct Hl as [Hd Hl].
+          destruct l.
+          + simpl in Hlast. inversion Hlast. clear Hlast. subst.
+            left. unfold Ensembles.In. apply Hd.
+          + right. unfold Ensembles.In.
+            pose proof (P := witnessing_sequence_extend).
+            destruct l as [|x' l'].
+            { simpl in Hlast. inversion Hlast. subst.
+              specialize (P d d m []).
+              destruct P as [_ P]. simpl in P.
+              simpl in Hl.
+              inversion Hl. subst. clear Hl.
+              assert (Hsomed: Some d = Some d).
+              { reflexivity. }
+              specialize (P (conj Hsomed Hwit')).
+              destruct P as [Hwitd [step' Hstep']].
+              exists step'. exists d.
+              destruct Hstep' as [Hstep' Hm].
+              split.
+              { apply Hstep'. }
+              split.
+              { apply IHlen. unfold witnessed_elements_of_max_len.
+                exists [d].
+                split.
+                2: { simpl. lia. }
+                unfold is_witnessing_sequence. simpl.
+                split.
+                { reflexivity. }
+                split.
+                { apply Hd. }
+                apply Forall_nil.
+                exact I.
+              }
+              apply Hm.
+            }
+            simpl in P.
+            simpl in Hlast.
+            simpl in Hl.
+            inversion Hl. subst. clear Hl.
+            inversion H2. subst. clear H2.
+            pose (mp := (rev (d0 :: x' :: l')) !! 1).
+            simpl in mp.
+            epose proof (Htot := (@list_lookup_lookup_total_lt (Domain M) _ (rev (d0 :: x' :: l')) 1 _)).
+            Unshelve. 2: { constructor. exact d0. }
+            2: { simpl. rewrite app_length. rewrite app_length. simpl.  lia.  }
+
+            remember (@lookup_total nat (@Domain Σ M) (list (@Domain Σ M))
+                 (@list_lookup_total (@Domain Σ M) {| inhabitant := d0 |}) (S O)
+                 (@rev (@Domain Σ M) (@cons (@Domain Σ M) d0 (@cons (@Domain Σ M) x' l')))) as mprev.
+
+            specialize (IHlen mprev).
+            unfold witnessed_elements_of_max_len in IHlen.
+            specialize (P mprev d m  (rev (tl (rev (d0::x'::l'))))).
+
+            assert (Heq1: d::d0::x'::l' = d::(rev (tail (rev (d0::x'::l')))) ++ [m]).
+            {
+              apply f_equal.
+              simpl.
+              assert (Hx'r: [x'] = rev [x']).
+              { reflexivity. }
+              rewrite Hx'r.
+              rewrite -rev_app_distr.
+              assert (Hd0r: [d0] = rev [d0]).
+              { reflexivity. }
+              rewrite Hd0r.
+              rewrite -rev_app_distr.
+              rewrite rev_tail_rev_app_last.
+              simpl.
+              apply Hlast.
+              reflexivity.
+            }
+            destruct P as [_ P].
+            
+
+            destruct (rev (tail (rev (d0 :: x' :: l')))) eqn:Heqrev.
+            {
+              apply length_zero_iff_nil in Heqrev.
+              rewrite rev_length in Heqrev.
+              apply length_tail_zero in Heqrev.
+              rewrite rev_length in Heqrev.
+              simpl in Heqrev. lia.
+            }
+
+            simpl in Heq1. inversion Heq1. subst d0. clear Heq1.
+            simpl in P.
+            rewrite -H2 in P.
+            
+            assert (Hm : (match l with [] => Some d1 | _ :: _ => last l end ) = Some mprev).
+            {
+              clear P Heqrev H1 H3 H4 mp.
+              destruct l.
+              { simpl in H2. inversion H2. subst. reflexivity. }
+              simpl.
+              simpl in H2.
+              inversion H2. subst x' l'. clear H2.
+              simpl in Htot.
+              destruct (l ++ [m]) eqn:Hcontra.
+              { pose proof (Hcontra' := @app_length _ l [m]).
+                rewrite Hcontra in Hcontra'.
+                simpl in Hcontra'. lia.
+              }
+              rewrite -Hcontra in Htot.
+              rewrite rev_app_distr in Htot. simpl in Htot.
+
+              destruct l.
+              { simpl in Htot. apply Htot. }
+              simpl in Htot.
+              rewrite -Htot.
+              rewrite hd_error_lookup.
+              rewrite hd_error_app. rewrite hd_error_app.
+              apply last_rev_head.
+            }
+            specialize (P (@conj _ _ Hm Hwit')). clear Hm Hwit'.
+            destruct P as [Hwitmprev [step' [Hstep' Hm]]].
+            exists step'. exists mprev.
+            split.
+            { apply Hstep'. }
+            split.
+            2: { apply Hm. }
+            apply IHlen.
+            exists (d::d1::l).
+            split.
+            { apply Hwitmprev. }
+            simpl. simpl in Hlen.
+            assert (Hlen': S (length l') <= len).
+            { lia. }
+            assert (length (l') = length (l)).
+            { apply (@list_len_slice _ _ _ _ _ H2). }
+            rewrite -H. lia.
+      Qed.
+      
+          
+      Lemma witnessed_elements_included_in_interp:
+        Included _ witnessed_elements (@pattern_interpretation Σ M ρₑ ρₛ patt_ind_gen).
+      Proof.
+        intros x H.
+        unfold Ensembles.In in H. unfold witnessed_elements in H.
+        destruct H as [wit Hwit].
+        assert (H': Ensembles.In (Domain M) (witnessed_elements_of_max_len (length wit)) x).
+        { unfold Ensembles.In. exists wit. split. apply Hwit. lia. }
+        destruct wit as [|y l'] eqn:Hl.
+        { unfold is_witnessing_sequence in Hwit. destruct Hwit. contradiction. }
+        eapply witnessed_elements_of_max_len_included_in_interp.
+        simpl in H'.
+        apply H'.
+      Qed.
+        
+      
       
       Lemma patt_ind_gen_simpl:
         @pattern_interpretation Σ M ρₑ ρₛ patt_ind_gen = witnessed_elements.
       Proof.
-      Abort.
+        apply Ensembles_Ext.eq_iff_Same_set.
+        split.
+        + apply interp_included_in_witnessed_elements.
+        + apply witnessed_elements_included_in_interp.
+      Qed.
 
     End with_interpretation.
   End inductive_generation.
